WIP

src/ModAdequacy.v
@@ -21,188 +21,6 @@ From Fairness Require Import SchedSim Adequacy.
 
 Set Implicit Arguments.
 
-Section AUX.
-
-  Lemma list_forall2_implies
-        A B (f1 f2: A -> B -> Prop) la lb
-        (FA: List.Forall2 f1 la lb)
-        (IMP: forall a b, (f1 a b) -> (f2 a b))
-    :
-    List.Forall2 f2 la lb.
-  Proof.
-    move FA before B. revert_until FA. induction FA; i; ss.
-    econs; eauto.
-  Qed.
-
-  Inductive Forall3 (A B C : Type) (R : A -> B -> C -> Prop) : list A -> list B -> list C -> Prop :=
-    Forall3_nil : Forall3 R [] [] []
-  | Forall3_cons : forall (x : A) (y : B) (z : C) (l1 : list A) (l2 : list B) (l3: list C),
-      R x y z -> Forall3 R l1 l2 l3 -> Forall3 R (x :: l1) (y :: l2) (z :: l3).
-
-  Lemma list_forall3_implies_forall2_3
-        A B C (f1: A -> B -> C -> Prop) (f2: A -> C -> Prop)
-        la lb lc
-        (FA: Forall3 f1 la lb lc)
-        (IMP: forall a b c, (f1 a b c) -> (f2 a c))
-    :
-    List.Forall2 f2 la lc.
-  Proof.
-    move FA before C. revert_until FA. induction FA; i; ss.
-    econs; eauto.
-  Qed.
-
-  Lemma list_forall3_implies_forall2_2
-        A B C (f1: A -> B -> C -> Prop) (f2: A -> B -> Prop)
-        la lb lc
-        (FA: Forall3 f1 la lb lc)
-        (IMP: forall a b c, (f1 a b c) -> (f2 a b))
-    :
-    List.Forall2 f2 la lb.
-  Proof.
-    move FA before C. revert_until FA. induction FA; i; ss.
-    econs; eauto.
-  Qed.
-
-  Import NatMap.
-  Import NatMapP.
-
-  Lemma nm_forall3_implies_find_some
-        elt1 elt2 elt3 (m1: NatMap.t elt1) (m2: NatMap.t elt2) (m3: NatMap.t elt3)
-        P
-        (FA: Forall3 (fun '(k1, e1) '(k2, e2) '(k3, e3) => (k1 = k2) /\ (k1 = k3) /\ (P e1 e2 e3 k1))
-                     (elements m1) (elements m2) (elements m3))
-    :
-    forall k e1 e2 e3 (FIND1: find k m1 = Some e1) (FIND2: find k m2 = Some e2) (FIND3: find k m3 = Some e3),
-      P e1 e2 e3 k.
-  Proof.
-    match goal with
-    | FA: Forall3 _ ?_ml1 ?_ml2 ?_ml3 |- _ => remember _ml1 as ml1; remember _ml2 as ml2; remember _ml3 as ml3
-    end.
-    move FA before elt3. revert_until FA. induction FA; i.
-    { symmetry in Heqml1; apply elements_Empty in Heqml1.
-      symmetry in Heqml2; apply elements_Empty in Heqml2.
-      symmetry in Heqml3; apply elements_Empty in Heqml3.
-      apply nm_empty_eq in Heqml1, Heqml2, Heqml3. subst. rewrite F.empty_o in FIND1; ss.
-    }
-    des_ifs. des; clarify. destruct (F.eq_dec k k2); clarify.
-    { eapply nm_elements_cons_find_some in Heqml1, Heqml2, Heqml3. clarify. }
-    hexploit nm_elements_cons_rm. eapply Heqml1. intro RM1.
-    hexploit nm_elements_cons_rm. eapply Heqml2. intro RM2.
-    hexploit nm_elements_cons_rm. eapply Heqml3. intro RM3.
-    eapply IHFA; eauto. rewrite nm_find_rm_neq; auto. rewrite nm_find_rm_neq; auto. rewrite nm_find_rm_neq; auto.
-  Qed.
-
-  Lemma nm_find_some_implies_forall3
-        elt1 elt2 elt3 (m1: NatMap.t elt1) (m2: NatMap.t elt2) (m3: NatMap.t elt3)
-        (P: elt1 -> elt2 -> elt3 -> key -> Prop)
-        (WFP1: nm_wf_pair m1 m2)
-        (WFP2: nm_wf_pair m1 m3)
-        (PROP: forall k e1 e2 e3
-                 (FIND1: find k m1 = Some e1) (FIND2: find k m2 = Some e2) (FIND3: find k m3 = Some e3), P e1 e2 e3 k)
-    :
-    Forall3 (fun '(k1, e1) '(k2, e2) '(k3, e3) => (k1 = k2) /\ (k1 = k3) /\ (P e1 e2 e3 k1))
-            (elements m1) (elements m2) (elements m3).
-  Proof.
-    remember (elements m1) as l1. move l1 before elt3. revert_until l1. induction l1; i; ss.
-    { symmetry in Heql1. apply elements_Empty in Heql1. dup Heql1.
-      hexploit nm_wf_pair_empty. eapply WFP1. i. apply H in Heql0. apply nm_empty_eq in Heql0. subst. rewrite elements_empty.
-      hexploit nm_wf_pair_empty. eapply WFP2. i. apply H0 in Heql1. apply nm_empty_eq in Heql1. subst. rewrite elements_empty.
-      econs.
-    }
-    destruct a as [k e1]. hexploit nm_elements_cons_rm. eauto. intros ELEM1. rewrite ELEM1 in Heql1.
-    destruct (elements m2) eqn:Heql2.
-    { exfalso. apply elements_Empty in Heql2. hexploit nm_wf_pair_empty. eapply WFP1. i. apply H in Heql2.
-      apply nm_empty_eq in Heql2. subst. rewrite elements_empty in Heql1. inv Heql1. }
-    destruct (elements m3) eqn:Heql3.
-    { exfalso. apply elements_Empty in Heql3. hexploit nm_wf_pair_empty. eapply WFP2. i. apply H in Heql3.
-      apply nm_empty_eq in Heql3. subst. rewrite elements_empty in Heql1. inv Heql1. }
-    destruct p as [k0 e2]. rename l into l2. symmetry in Heql2.
-    destruct p0 as [k1 e3]. rename l0 into l3. symmetry in Heql3.
-    hexploit nm_elements_cons_rm. eapply Heql2. intro ELEM2. rewrite ELEM2 in Heql2.
-    hexploit nm_elements_cons_rm. eapply Heql3. intro ELEM3. rewrite ELEM3 in Heql3.
-    assert (k = k0).
-    { hexploit nm_wf_pair_elements_forall2. eapply WFP1. rewrite <- Heql1, <- Heql2. i. inv H. auto. }
-    assert (k = k1).
-    { hexploit nm_wf_pair_elements_forall2. eapply WFP2. rewrite <- Heql1, <- Heql3. i. inv H0. auto. }
-    replace k0 with k in *. replace k1 with k in *. clear H H0. econs.
-    2:{ rewrite ELEM2, ELEM3. eapply IHl1; eauto.
-        apply nm_wf_pair_rm; auto. apply nm_wf_pair_rm; auto.
-        i. eapply PROP.
-        rewrite F.remove_o in FIND1. des_ifs. rewrite F.remove_o in FIND2. des_ifs. rewrite F.remove_o in FIND3. des_ifs.
-    }
-    splits; auto. eapply PROP. all: eapply nm_elements_cons_find_some; eauto.
-  Qed.
-
-  Inductive Forall4 (A B C D : Type) (R : A -> B -> C -> D -> Prop) : list A -> list B -> list C -> list D -> Prop :=
-    Forall4_nil : Forall4 R [] [] [] []
-  | Forall4_cons : forall (x : A) (y : B) (z : C) (w : D) (l1 : list A) (l2 : list B) (l3: list C) (l4: list D),
-      R x y z w -> Forall4 R l1 l2 l3 l4 -> Forall4 R (x :: l1) (y :: l2) (z :: l3) (w :: l4).
-
-  Lemma list_forall4_implies_forall2_4
-        A B C D (f1: A -> B -> C -> D -> Prop) (f2: A -> D -> Prop)
-        la lb lc ld
-        (FA: Forall4 f1 la lb lc ld)
-        (IMP: forall a b c d, (f1 a b c d) -> (f2 a d))
-    :
-    List.Forall2 f2 la ld.
-  Proof.
-    move FA before D. revert_until FA. induction FA; i; ss. econs; eauto.
-  Qed.
-
-  Lemma list_forall4_implies_forall2_3
-        A B C D (f1: A -> B -> C -> D -> Prop) (f2: A -> C -> Prop)
-        la lb lc ld
-        (FA: Forall4 f1 la lb lc ld)
-        (IMP: forall a b c d, (f1 a b c d) -> (f2 a c))
-    :
-    List.Forall2 f2 la lc.
-  Proof.
-    move FA before D. revert_until FA. induction FA; i; ss. econs; eauto.
-  Qed.
-
-  Lemma list_forall4_implies_forall2_2
-        A B C D (f1: A -> B -> C -> D -> Prop) (f2: A -> B -> Prop)
-        la lb lc ld
-        (FA: Forall4 f1 la lb lc ld)
-        (IMP: forall a b c d, (f1 a b c d) -> (f2 a b))
-    :
-    List.Forall2 f2 la lb.
-  Proof.
-    move FA before D. revert_until FA. induction FA; i; ss. econs; eauto.
-  Qed.
-
-  Import NatMap.
-  Import NatMapP.
-
-  Lemma nm_forall4_implies_find_some
-        elt1 elt2 elt3 elt4 (m1: NatMap.t elt1) (m2: NatMap.t elt2) (m3: NatMap.t elt3) (m4: NatMap.t elt4)
-        P
-        (FA: Forall4 (fun '(k1, e1) '(k2, e2) '(k3, e3) '(k4, e4) => (k1 = k2) /\ (k1 = k3) /\ (k1 = k4) /\ (P e1 e2 e3 e4 k1))
-                     (elements m1) (elements m2) (elements m3) (elements m4))
-    :
-    forall k e1 e2 e3 e4
-      (FIND1: find k m1 = Some e1) (FIND2: find k m2 = Some e2) (FIND3: find k m3 = Some e3) (FIND4: find k m4 = Some e4),
-      P e1 e2 e3 e4 k.
-  Proof.
-    match goal with
-    | FA: Forall4 _ ?_ml1 ?_ml2 ?_ml3 ?_ml4 |- _ =>
-        remember _ml1 as ml1; remember _ml2 as ml2; remember _ml3 as ml3; remember _ml4 as ml4
-    end.
-    move FA before elt4. revert_until FA. induction FA; i.
-    { symmetry in Heqml1; apply elements_Empty in Heqml1.
-      apply nm_empty_eq in Heqml1. subst. rewrite F.empty_o in FIND1; ss.
-    }
-    des_ifs. des; clarify. destruct (F.eq_dec k k3); clarify.
-    { eapply nm_elements_cons_find_some in Heqml1, Heqml2, Heqml3, Heqml4. clarify. }
-    hexploit nm_elements_cons_rm. eapply Heqml1. intro RM1.
-    hexploit nm_elements_cons_rm. eapply Heqml2. intro RM2.
-    hexploit nm_elements_cons_rm. eapply Heqml3. intro RM3.
-    hexploit nm_elements_cons_rm. eapply Heqml4. intro RM4.
-    eapply IHFA; eauto. all: rewrite nm_find_rm_neq; auto.
-  Qed.
-
-End AUX.
-
 
 
 Section LADEQ.
@@ -665,3 +483,77 @@ Section ADEQ.
   Qed.
 
 End ADEQ.
+
+
+
+Section USERADEQ.
+
+  Theorem usersim_adequacy
+          m_src m_tgt
+          p_src p_tgt
+          (MSIM: ModSim.UserSim.sim m_src m_tgt p_src p_tgt)
+    :
+    forall tid,
+      Adequacy.improves (interp_all m_src.(Mod.st_init) p_src tid)
+                        (interp_all m_tgt.(Mod.st_init) p_tgt tid).
+  Proof.
+    apply modsim_implies_yord_mod in MSIM.
+    apply yord_implies_stid_mod in MSIM.
+    apply stid_implies_nosync_mod in MSIM.
+    apply nosync_implies_stutter_mod in MSIM.
+    inv MSIM. i.
+    eapply Adequacy.adequacy. eapply wf_tgt_inhabited. eapply wf_tgt_open.
+    instantiate (1:=wf_src).
+    destruct (mod_funs_cases m_src).
+    { ii. specialize (init mt). des. exists im_src, false, false.
+      destruct (Th.find tid (prog2ths m_src p)) eqn:FIND.
+      2:{ unfold interp_all. rewrite unfold_interp_sched_nondet_None.
+          rewrite interp_state_vis. rewrite <- bind_trigger. pfold. econs 10. auto.
+      }
+      unfold interp_all. erewrite unfold_interp_sched_nondet_Some.
+      2: eauto.
+      assert (UB: i = (Vis (inl1 (inl1 Undefined)) (Empty_set_rect _))).
+      { revert_until funs. clear. i. unfold prog2ths, numbering in FIND.
+        remember 0 as k. clear Heqk. move p after tid. revert_until p. induction p; i; ss.
+        destruct a as [fn args]. unfold NatMapP.uncurry in FIND. ss.
+        destruct (tid_dec tid k); clarify.
+        { rewrite nm_find_add_eq in FIND. clarify. unfold fn2th. rewrite H. auto. }
+        rewrite nm_find_add_neq in FIND; auto. eapply IHp; eauto.
+      }
+      clarify. rewrite interp_thread_vis_eventE. ired. rewrite interp_state_vis.
+      rewrite <- bind_trigger. pfold. econs 10.
+    }
+
+    des. rename fn into fn0, ktr into ktr0, H into SOME0.
+    eapply ModSimStutter_local_sim_implies_gsim. 3: eapply init.
+    instantiate (1:= fun o0 => @epsilon _ wf_tgt_inhabited (fun o1 => wf_tgt.(lt) o0 o1)).
+    { i. hexploit (@epsilon_spec _ wf_tgt_inhabited (fun o1 => wf_tgt.(lt) t o1)); eauto. }
+    instantiate (1:=wf_stt).
+    unfold ModSimStutter_local_sim_threads, prog2ths. unfold numbering.
+    remember 0 as k. clear Heqk. move p before k. revert_until p.
+    induction p; i.
+    { ss. unfold NatMap.Raw.empty. econs. }
+    rewrite !map_cons, !_numbering_cons. destruct a as [fn args].
+    rewrite !of_list_cons. eapply nm_find_some_implies_forall2.
+    { apply nm_wf_pair_add. clear. move p after m_src. revert_until p. induction p; i.
+      { ss. apply nm_wf_pair_empty_empty_eq. }
+      ss. destruct a as [fn args]. unfold NatMapP.uncurry. ss. eapply nm_wf_pair_add.
+      eauto.
+    }
+    i. destruct (tid_dec k k0); clarify.
+    { clear IHp. rewrite nm_find_add_eq in FIND1, FIND2. clarify. unfold fn2th.
+      dup funs. specialize (funs0 fn0 ([]: list Val)↑). rewrite SOME0 in funs0.
+      specialize (funs fn args). des_ifs; ss.
+      unfold local_sim in funs0. ii.
+      specialize (funs0 _ _ _ _ _ _ _ INV _ _ THS VALID _ UPD). des.
+      esplits; eauto. i. specialize (funs0 _ _ _ _ _ _ _ INV1 VALID1 _ TGT). des.
+      esplits. eapply SRC. i. instantiate (1:=o).
+      pfold. eapply pind6_fold. rewrite <- bind_trigger. econs 7.
+    }
+    rewrite nm_find_add_neq in FIND1, FIND2; auto.
+    specialize (IHp (S k)). eapply nm_forall2_implies_find_some in IHp; eauto.
+  Qed.
+
+
+
+End USERADEQ.
